typo

hax-lib/proofs/fstar/extraction/Hax_lib.Prop.fst
@@ -2,4 +2,13 @@ module Hax_lib.Prop
 
 type t_Prop = Type0
 
-unfold let implies #a #b (lhs: t_Prop) (rhs: (x:unit{lhs} -> t_Prop)): t_Prop = (~ lhs) \/ rhs ()
+val v_assert (p: t_Prop) : Pure unit (requires p) (ensures (fun x -> p))
+let v_assert (v__formula: t_Prop) = ()
+
+val v_assume (p: t_Prop) : Pure unit (requires True) (ensures (fun x -> p))
+let v_assume (v__formula: t_Prop) = assume v__formula
+
+
+unfold let v_exists (v__f: 'a -> t_Prop): t_Prop = exists (x: 'a). v__f x
+unfold let v_forall (v__f: 'a -> t_Prop): t_Prop = forall (x: 'a). v__f x
+unfold let implies (lhs: t_Prop) (rhs: (x:unit{lhs} -> t_Prop)): t_Prop = (~ lhs) \/ rhs ()
